SeqExt.dfy
@@ -1,11 +1,19 @@
 module SeqExt {
-  import Seq = Std.Collections.Seq
+    import Seq = Std.Collections.Seq
+    import Functions = Std.Functions
 
-  lemma LemmaToSetAdds<X>(xs: seq<X>, ys: seq<X>)
-    ensures Seq.ToSet(xs) + Seq.ToSet(ys) == Seq.ToSet(xs + ys)
-  {
-    reveal Seq.ToSet();
-    assert forall x :: x in (xs + ys) <==> (x in xs) || (x in ys);
-  }
-        
+    lemma LemmaToSetAdds<X>(xs: seq<X>, ys: seq<X>)
+        ensures Seq.ToSet(xs) + Seq.ToSet(ys) == Seq.ToSet(xs + ys)
+    {
+        reveal Seq.ToSet();
+        assert forall x :: x in (xs + ys) <==> (x in xs) || (x in ys);
+    }
+
+    lemma MapConservesNoDuplicates<X, Y>(f: X -> Y, xs: seq<X>)
+        requires Seq.HasNoDuplicates(xs)
+        requires Functions.Injective(f)
+        ensures Seq.HasNoDuplicates(Seq.Map(f, xs))
+    {
+        reveal Seq.HasNoDuplicates();
+    }
 }
